src/absyn/syntax.fsi
@@ -233,12 +233,12 @@ type monad_abbrev = {
   parms:binders;
   def:typ
   }
-type sub_effect = {
+type sub_eff = {
   source:lident;
   target:lident;
   lift: typ
  }
-type new_effect = {
+type eff_decl = {
     mname:lident;
     binders:binders;
     qualifiers:list<qualifier>;
@@ -268,8 +268,8 @@ and sigelt =
   | Sig_let            of letbindings * Range.range * list<lident> * list<qualifier>
   | Sig_main           of exp * Range.range 
   | Sig_bundle         of list<sigelt> * Range.range * list<lident> (* an inductive type is a bundle of all mutually defined Sig_tycons and Sig_datacons *)
-  | Sig_new_effect     of new_effect * Range.range
-  | Sig_sub_effect     of sub_effect * Range.range
+  | Sig_new_effect     of eff_decl * Range.range
+  | Sig_sub_effect     of sub_eff * Range.range
   | Sig_effect_abbrev  of lident * binders * comp * list<qualifier> * Range.range
   | Sig_pragma         of pragma * Range.range
 type sigelts = list<sigelt>
