lib/ghost.fst
@@ -14,22 +14,12 @@
    limitations under the License.
 *)
 (*
-  This module provides
-     1. A GHOST effect, to encapsulate irrelevant computations
-     2. A ghost type, to abstract computationally irrelevant values
+  This module provides a ghost type,
+  to abstract computationally irrelevant values.
+
+  It relies on the GHOST effect defined in Prims
 *)
 module Ghost
-total new_effect GHOST = PURE
-
-sub_effect
-  PURE ~> GHOST = fun (a:Type) (wp:PureWP a) -> wp
-
-effect GTot (a:Type) = GHOST a (pure_null_wp a) (pure_null_wp a)
-effect Ghost (a:Type) (pre:Type) (post:PurePost a) =
-       GHOST a
-           (fun (p:PurePost a) -> pre /\ (forall (x:a). post x ==> p x))
-           (fun (p:PurePost a) -> forall (x:a). pre /\ post x ==> p x)
-
 private type ghost (a:Type) = a
 val reveal: #a:Type -> ghost a -> GTot a
 let reveal x = x
@@ -42,8 +32,9 @@ val lemma_hide_reveal: #a:Type
                    -> Lemma (ensures (hide (reveal x) = x))
 let lemma_hide_reveal x = ()
 
-assume val as_ghost: #a:Type
+val as_ghost: #a:Type
           -> f:(unit -> Tot a)
           -> Pure (ghost a)
                   (requires True)
                   (ensures (fun x -> reveal x = f ()))
+let as_ghost f = f ()
